theories/interop/basics_resources.v
@@ -1,0 +1,219 @@
+From Coq Require Import ssreflect.
+From stdpp Require Import strings gmap.
+From iris.base_logic.lib Require Import ghost_map ghost_var.
+From iris.proofmode Require Import proofmode.
+From melocoton Require Import named_props.
+From melocoton.interop Require Export basics.
+
+Section BasicsResources.
+Context {Σ : gFunctors}.
+Context {llocmapGS: ghost_mapG Σ lloc lloc_visibility}.
+Context {lstoreGS: ghost_mapG Σ lloc block}.
+
+(* Ghost state for [lloc_map] *)
+
+Definition lloc_own_priv (γGS : gname) (γ : lloc) : iProp Σ :=
+  γ ↪[γGS] LlocPrivate.
+
+Definition lloc_own_pub (γGS : gname) (γ : lloc) (ℓ : loc) : iProp Σ :=
+  γ ↪[γGS]□ LlocPublic ℓ.
+
+Instance lloc_own_pub_persistent γGS γ ℓ : Persistent (lloc_own_pub γGS γ ℓ).
+Proof using. apply _. Qed.
+
+Definition lloc_own_auth (γGS : gname) (χ : lloc_map) : iProp Σ :=
+  "Hχgmap" ∷ ghost_map_auth γGS 1 χ ∗
+  "Hχpubs" ∷ ([∗ map] γ↦ℓ ∈ (lloc_map_pubs χ), lloc_own_pub γGS γ ℓ).
+
+Lemma lloc_own_auth_get_pub_all γGS χ :
+  lloc_own_auth γGS χ -∗
+  [∗ map] γ↦ℓ ∈ (lloc_map_pubs χ), lloc_own_pub γGS γ ℓ.
+Proof using.
+  iNamed 1. iApply "Hχpubs".
+Qed.
+
+Lemma lloc_own_auth_get_pub γGS χ γ ℓ :
+  χ !! γ = Some (LlocPublic ℓ) →
+  lloc_own_auth γGS χ -∗
+  lloc_own_pub γGS γ ℓ.
+Proof using.
+  intros Hγ. iNamed 1.
+  iDestruct (big_sepM_lookup with "Hχpubs") as "?"; eauto.
+Qed.
+
+Lemma lloc_own_pub_of γGS χ γ ℓ :
+  lloc_own_auth γGS χ -∗
+  lloc_own_pub γGS γ ℓ -∗
+  ⌜χ !! γ = Some (LlocPublic ℓ)⌝.
+Proof using.
+  iIntros "Hχ Hpub". iNamed "Hχ".
+  by iDestruct (ghost_map_lookup with "Hχgmap Hpub") as %?.
+Qed.
+
+Lemma lloc_own_priv_of γGS χ γ :
+  lloc_own_auth γGS χ -∗
+  lloc_own_priv γGS γ -∗
+  ⌜χ !! γ = Some LlocPrivate⌝.
+Proof using.
+  iIntros "Hχ Hpub". iNamed "Hχ".
+  by iDestruct (ghost_map_lookup with "Hχgmap Hpub") as %?.
+Qed.
+
+Lemma lloc_own_expose γGS χ γ ℓ :
+  lloc_own_auth γGS χ -∗
+  lloc_own_priv γGS γ ==∗
+  lloc_own_auth γGS (<[γ:=LlocPublic ℓ]> χ) ∗ lloc_own_pub γGS γ ℓ.
+Proof using.
+  iIntros "Hχ Hγ".
+  iDestruct (lloc_own_priv_of with "Hχ Hγ") as %Hχγ.
+  iNamed "Hχ".
+  iMod (ghost_map_update with "Hχgmap Hγ") as "[$ Hγ]".
+  iMod (ghost_map_elem_persist with "Hγ") as "#Hγ".
+  iFrame "Hγ". iModIntro.
+  rewrite lloc_map_pubs_insert_pub.
+  iApply big_sepM_insert; eauto.
+  apply lloc_map_pubs_lookup_None; eauto.
+Qed.
+
+(* Ghost state for [lstore] *)
+
+Definition lstore_own_elem (γGS : gname) (γ : lloc) (dq : dfrac) (b : block) :=
+  match mutability b with
+  | Mut => γ ↪[γGS]{dq} b
+  | Immut => γ ↪[γGS]□ b
+  end%I.
+
+Definition lstore_own_mut (γGS : gname) (γ : lloc) (dq : dfrac) (b : block) :=
+  (lstore_own_elem γGS γ dq b ∗ ⌜mutability b = Mut⌝)%I.
+
+Definition lstore_own_immut (γGS : gname) (γ : lloc) (b : block) :=
+  (lstore_own_elem γGS γ (DfracOwn 1) b ∗ ⌜mutability b = Immut⌝)%I.
+
+Definition lstore_own_auth (γGS : gname) (ζ : lstore) : iProp Σ :=
+  "Hζgmap" ∷ ghost_map_auth γGS 1 ζ ∗
+  "#Hζimmut" ∷ ([∗ map] γ↦b ∈ (lstore_immut_blocks ζ), lstore_own_immut γGS γ b).
+
+Global Instance lstore_own_immut_persistent γGS γ b :
+  Persistent (lstore_own_immut γGS γ b).
+Proof using.
+  unfold Persistent.
+  iIntros "[? %H]". unfold lstore_own_immut, lstore_own_elem.
+  rewrite H. rewrite bi.persistently_sep bi.persistently_pure.
+  iSplit; auto. by iApply persistent.
+Qed.
+
+Lemma lstore_own_elem_to_mut γGS γ dq b :
+  mutability b = Mut →
+  lstore_own_elem γGS γ dq b -∗
+  lstore_own_mut γGS γ dq b.
+Proof using. intros H. rewrite /lstore_own_mut /lstore_own_elem H. eauto. Qed.
+
+Lemma lstore_own_mut_to_elem γGS γ dq b :
+  lstore_own_mut γGS γ dq b -∗
+  lstore_own_elem γGS γ dq b.
+Proof using. by iIntros "[? _]". Qed.
+
+Lemma lstore_own_elem_to_immut γGS γ dq b :
+  mutability b = Immut →
+  lstore_own_elem γGS γ dq b -∗
+  lstore_own_immut γGS γ b.
+Proof using. intros H. rewrite /lstore_own_immut /lstore_own_elem H. eauto. Qed.
+
+Lemma lstore_own_immut_to_elem γGS γ b :
+  lstore_own_immut γGS γ b -∗
+  lstore_own_elem γGS γ (DfracOwn 1) b.
+Proof using. by iIntros "[? _]". Qed.
+
+Lemma lstore_own_auth_get_immut_all γGS ζ :
+  lstore_own_auth γGS ζ -∗
+  [∗ map] γ↦b ∈ (lstore_immut_blocks ζ), lstore_own_immut γGS γ b.
+Proof using.
+  iNamed 1. iApply "Hζimmut".
+Qed.
+
+Lemma lstore_own_auth_get_immut γGS ζ γ b :
+  ζ !! γ = Some b →
+  mutability b = Immut →
+  lstore_own_auth γGS ζ -∗
+  lstore_own_immut γGS γ b.
+Proof using.
+  intros ? ?. iNamed 1.
+  iDestruct (big_sepM_lookup with "Hζimmut") as "?"; eauto.
+  by eapply lstore_immut_blocks_lookup_immut.
+Qed.
+
+Lemma lstore_own_elem_of γGS ζ γ dq b :
+  lstore_own_auth γGS ζ -∗
+  lstore_own_elem γGS γ dq b -∗
+  ⌜ζ !! γ = Some b⌝.
+Proof using.
+  iNamed 1. iIntros "He".
+  destruct (mutability b) eqn:Hmut; rewrite /lstore_own_elem Hmut;
+    by iDestruct (ghost_map_lookup with "Hζgmap He") as %?.
+Qed.
+
+Lemma lstore_own_mut_of γGS ζ γ dq b :
+  lstore_own_auth γGS ζ -∗
+  lstore_own_mut γGS γ dq b -∗
+  ⌜ζ !! γ = Some b ∧ mutability b = Mut⌝.
+Proof using.
+  iIntros "Ha [H %]".
+  by iDestruct (lstore_own_elem_of with "Ha H") as %?.
+Qed.
+
+Lemma lstore_own_immut_of γGS ζ γ b :
+  lstore_own_auth γGS ζ -∗
+  lstore_own_immut γGS γ b -∗
+  ⌜ζ !! γ = Some b ∧ mutability b = Immut⌝.
+Proof using.
+  iIntros "Ha [H %]".
+  by iDestruct (lstore_own_elem_of with "Ha H") as %?.
+Qed.
+
+Lemma lstore_own_insert γGS ζ γ b :
+  ζ !! γ = None →
+  lstore_own_auth γGS ζ ==∗
+  lstore_own_auth γGS (<[γ:=b]> ζ) ∗ lstore_own_elem γGS γ (DfracOwn 1) b.
+Proof using.
+  iIntros (Hγ). iNamed 1.
+  iMod (ghost_map_insert _ b with "Hζgmap") as "[Hζgmap Helt]"; eauto.
+  iFrame "Hζgmap".
+  destruct (mutability b) eqn:Hmut.
+  { rewrite /lstore_own_elem Hmut. iFrame "Helt".
+    rewrite lstore_immut_blocks_insert_mut // delete_notin //; eauto. }
+  { iMod (ghost_map_elem_persist with "Helt") as "#Helt".
+    rewrite /lstore_own_elem Hmut. iFrame "Helt".
+    iModIntro. rewrite lstore_immut_blocks_insert_immut // big_sepM_insert; eauto.
+    iFrame. rewrite /lstore_own_immut /lstore_own_elem Hmut //. eauto. }
+Qed.
+
+Lemma lstore_own_update γGS ζ γ b b' :
+  lstore_own_auth γGS ζ -∗
+  lstore_own_mut γGS γ (DfracOwn 1) b ==∗
+  lstore_own_auth γGS (<[γ:=b']> ζ) ∗ lstore_own_elem γGS γ (DfracOwn 1) b'.
+Proof using.
+  iIntros "Ha He". iDestruct (lstore_own_mut_of with "Ha He") as %[? _].
+  iNamed "Ha". iDestruct "He" as "[He %Hmut]".
+  rewrite /lstore_own_elem Hmut.
+  iMod (ghost_map_update with "Hζgmap He") as "[Hζgmap He]".
+  destruct (mutability b') eqn:Hmut'.
+  { iFrame. iApply (big_sepM_subseteq with "Hζimmut").
+    rewrite lstore_immut_blocks_insert_mut //. apply delete_subseteq. }
+  { iMod (ghost_map_elem_persist with "He") as "#$". iFrame.
+    rewrite lstore_immut_blocks_insert_immut //.
+    iApply big_sepM_insert; eauto. iModIntro.
+    rewrite /lstore_own_immut /lstore_own_elem Hmut'; eauto. }
+Qed.
+
+Lemma lstore_own_delete γGS ζ γ b :
+  lstore_own_auth γGS ζ -∗
+  lstore_own_mut γGS γ (DfracOwn 1) b ==∗
+  lstore_own_auth γGS (delete γ ζ).
+Proof using.
+  iNamed 1. iIntros "[He %Hmut]". rewrite /lstore_own_elem Hmut.
+  iMod (ghost_map_delete with "Hζgmap He") as "Hζgmap". iFrame.
+  rewrite lstore_immut_blocks_delete.
+  iApply (big_sepM_subseteq with "Hζimmut"). apply delete_subseteq.
+Qed.
+
+End BasicsResources.
