theories/interop/wrapper_wp_update_laws.v
@@ -10,7 +10,7 @@ From iris.algebra Require Import gset gset_bij.
 From iris.proofmode Require Import proofmode.
 From melocoton.c_toy_lang Require Import lang melocoton.lang_instantiation melocoton.primitive_laws.
 From melocoton.ml_toy_lang Require Import lang melocoton.lang_instantiation melocoton.primitive_laws.
-From melocoton.interop Require Import linking_wp basics wrapper_wp wrapper_wp_block_sim.
+From melocoton.interop Require Import linking_wp basics basics_resources wrapper_wp wrapper_wp_block_sim.
 Import Wrap.
 
 Section UpdateLaws.
@@ -29,7 +29,7 @@ Implicit Types P : iProp Σ.
 Context (σ : Wrap.state).
 Notation SI := (weakestpre.state_interp σ).
 
-Lemma ml_to_mut θ l vs: ⊢ (GC θ ∗ l ↦∗ vs ∗ SI ==∗ SI ∗ GC θ ∗ ∃ b γ, γ ↦mut{DfracOwn 1} (TagDefault,b) ∗ block_sim_raw l γ ∗ block_sim_arr vs b)%I.
+Lemma ml_to_mut θ l vs: ⊢ (GC θ ∗ l ↦∗ vs ∗ SI ==∗ SI ∗ GC θ ∗ ∃ b γ, γ ↦mut (TagDefault,b) ∗ block_sim_raw l γ ∗ block_sim_arr vs b)%I.
 Proof.
   iIntros "(HGC & Hl & Hσ)".
   iDestruct (GC_in_C with "Hσ HGC") as "%H"; destruct H as (ρc & mem & ->).
@@ -39,18 +39,19 @@ Proof.
     [apply Hstore_blocks|apply Hlσ|..].
   iMod (gen_heap_update _ _ _ None with "HAσMLv Hl") as "[HAσMLv Hl]".
   apply elem_of_dom in Hllζ. destruct Hllζ as [bb Hζσll].
-  iMod (ghost_map_insert _ bb with "HAζbl") as "(HAζbl & Hzz)".
-  1: { eapply map_disjoint_Some_l; done. }
-  iModIntro. iFrame "HGC".
   assert (ζfreeze !! ll = Some bb) as Hfreezell.
   1: { rewrite Hfreezeeq. by apply lookup_union_Some_l. }
   unfold is_store in Hstore.
   specialize (Hstore l vs ll bb Hlσ Hlχ Hfreezell) as Hstorel.
   inversion Hstorel; subst vs0 bb.
   iAssert (block_sim_arr vs lvs) as "#Hblock".
-  1: by iApply (block_sim_arr_of_ghost_state with "HAχvirt HAζpers").
+  1: by iApply (block_sim_arr_of_ghost_state with "HAχvirt HAζrest").
   iAssert (block_sim_raw l ll) as "#Hraw".
   1: by iApply (lloc_own_auth_get_pub with "HAχvirt").
+  iMod (lstore_own_insert _ _ ll (Mut, _) with "HAζrest") as "(HAζrest & Hzz)".
+  1: { eapply map_disjoint_Some_l; done. }
+  iDestruct (lstore_own_elem_to_mut with "Hzz") as "Hzz"; first done.
+  iModIntro. iFrame "HGC".
   assert (ζrest !! ll = None) as HζllNone.
   1: eapply map_disjoint_Some_l; done.
   iSplitR "Hzz". 1: iSplitL "HσC HnC".
@@ -62,38 +63,32 @@ Proof.
          rewrite dom_insert_L. eapply elem_of_dom_2 in Hlσ. set_solver. }
     iSplitL.
     { rewrite (pub_locs_in_lstore_insert_lstore_pub _ _ _ l) //.
-      iApply big_sepM_insert; [| by iFrame].
-      apply map_filter_lookup_None. right. intros ? ?%lloc_map_pubs_lookup_Some ?.
-      simplify_map_eq. by apply not_elem_of_dom in HζllNone. }
-    iSplitL.
-    { rewrite lstore_immut_blocks_insert_mut //. }
-    iPureIntro. split_and!.
-    all: eauto.
+      iApply big_sepM_insert; eauto. by iFrame. }
+    iPureIntro. split_and!; eauto.
     - symmetry. subst. by apply union_delete_insert.
     - apply map_disjoint_insert_r_2. 1: apply lookup_delete.
       apply map_disjoint_delete_l. done.
     - eapply is_store_blocks_discard_loc; eauto.
     - eapply is_store_discard_loc; eauto.
-  + iExists lvs, ll. cbn. iFrame. iFrame "Hblock Hraw".
-    iExists _; iApply "Hraw".
+  + iExists lvs, ll. eauto.
 Qed.
 
-Lemma mut_to_ml γ vs b θ: ⊢ (SI ∗ GC θ ∗ γ ↦mut{DfracOwn 1} (TagDefault,b) ∗ block_sim_arr vs b ==∗ SI ∗ GC θ ∗ ∃ l, l ↦∗ vs ∗ block_sim_raw l γ)%I.
+Lemma mut_to_ml γ vs b θ: ⊢ (SI ∗ GC θ ∗ γ ↦mut (TagDefault,b) ∗ block_sim_arr vs b ==∗ SI ∗ GC θ ∗ ∃ l, l ↦∗ vs ∗ block_sim_raw l γ)%I.
 Proof.
   iIntros "(Hσ & HGC & (Hl & (%ℓ & #Hlℓ)) & #Hsim)".
   iDestruct (GC_in_C with "Hσ HGC") as "%H"; destruct H as (ρc & mem & ->).
   iNamed "Hσ". iNamed "SIC".
-  iPoseProof (block_sim_arr_to_ghost_state with "HAχvirt HAζbl [] [] [] [] Hsim ") as "%Hsim".
+  iDestruct (block_sim_arr_to_ghost_state with "HAχvirt HAζrest [] [] [] [] Hsim") as %Hsim.
   1-4: iPureIntro; done.
   iPoseProof (lloc_own_pub_of with "HAχvirt Hlℓ") as "%Hχℓ".
   unfold is_store in Hstore.
-  iPoseProof (ghost_map_lookup with "HAζbl Hl") as "%Hζl".
+  iDestruct (lstore_own_mut_of with "HAζrest Hl") as %[Hζl _].
   iDestruct (big_sepM_delete _ _ _ ℓ with "HAχNone") as "[Hℓ HAχNone]".
   { eapply map_filter_lookup_Some. rewrite lloc_map_pubs_lookup_Some.
     split; eauto. by eapply elem_of_dom_2. }
   iDestruct (gen_heap_valid with "HAσMLv Hℓ") as "%Hlσ".
   iMod (gen_heap_update _ _ _ (Some vs) with "HAσMLv Hℓ") as "[HAσMLv Hℓ]".
-  iMod (ghost_map_delete with "HAζbl Hl") as "HAζbl".
+  iMod (lstore_own_delete with "HAζrest Hl") as "HAζrest".
   iModIntro. iFrame "HGC". iSplitR "Hℓ". 2: iExists ℓ; iFrame; done.
   cbn. iSplitL "HσC HnC".
   1: iExists _; iFrame.
@@ -101,10 +96,9 @@ Proof.
   iExists ζfreeze, (<[γ:=(Mut, (TagDefault, b))]>ζσ), (delete γ ζrest).
   iExists χvirt, (<[ ℓ := Some vs ]> σMLvirt).
   iFrame.
-  iSplitL "HAnMLv HAσdom". 2: iSplitL. 3: iSplitL. 4: iPureIntro; split_and!; eauto.
+  iSplitL "HAnMLv HAσdom". 2: iSplitL. 3: iPureIntro; split_and!; eauto.
   + iExists _; iFrame. iApply (dom_auth_dom with "HAσdom"); erewrite dom_insert_L; eapply elem_of_dom_2 in Hlσ; set_solver.
   + rewrite pub_locs_in_lstore_delete_lstore //.
-  + rewrite /lstore_immut_blocks map_filter_delete_not //. naive_solver.
   + erewrite (union_insert_delete ζσ ζrest). 2: eapply map_disjoint_Some_r. all: eauto.
   + apply map_disjoint_insert_l_2. 1: apply lookup_delete.
     apply map_disjoint_delete_r. done.
@@ -114,12 +108,12 @@ Proof.
     by constructor.
 Qed.
 
-Lemma freeze_to_mut γ bb θ: ⊢ (SI ∗ GC θ ∗ γ ↦fresh{DfracOwn 1} bb ==∗ SI ∗ GC θ ∗ γ ↦mut{DfracOwn 1} bb)%I.
+Lemma freeze_to_mut γ bb θ: ⊢ (SI ∗ GC θ ∗ γ ↦fresh bb ==∗ SI ∗ GC θ ∗ γ ↦mut bb)%I.
 Proof.
   iIntros "(Hσ & HGC & (Hmtζ & Hmtfresh))".
   iDestruct (GC_in_C with "Hσ HGC") as "%H"; destruct H as (ρc & mem & ->).
   iNamed "Hσ". iNamed "SIC".
-  iPoseProof (ghost_map_lookup with "HAζbl Hmtζ") as "%Hζγ".
+  iDestruct (lstore_own_mut_of with "HAζrest Hmtζ") as %[Hζγ _].
   pose (fresh_locs (lloc_map_pub_locs χvirt)) as ℓ.
   assert (ℓ ∉ lloc_map_pub_locs χvirt).
   { intros Hℓ. apply (fresh_locs_fresh (lloc_map_pub_locs χvirt) 0 ltac:(lia)).
@@ -143,9 +137,8 @@ Proof.
   unfold C_state_interp, named.
   iExists ζfreeze, ζσ, ζrest.
   iExists (<[γ:=LlocPublic ℓ]> χvirt), (<[ ℓ := None ]> σMLvirt).
-  iFrame. iFrame "HAζpers".
-  iSplitL "HAnMLv". 2: iSplitL. 3: iPureIntro; split_and!; eauto.
-  + iExists nMLv; iFrame.
+  iFrame.
+  iSplitL "HAnMLv"; eauto. iSplitL. 2: iPureIntro; split_and!; eauto.
   + rewrite pub_locs_in_lstore_insert_pub //. by eapply elem_of_dom_2.
   + eapply is_store_blocks_expose_lloc; eauto.
   + eapply is_store_expose_lloc; eauto.
@@ -156,31 +149,23 @@ Proof.
     - by eapply Hfreezeχ.
 Qed.
 
-Lemma freeze_to_immut γ bb θ: ⊢ (SI ∗ GC θ ∗ γ ↦fresh{DfracOwn 1} bb ==∗ SI ∗ GC θ ∗ γ ↦imm bb)%I.
+Lemma freeze_to_immut γ bb θ: ⊢ (SI ∗ GC θ ∗ γ ↦fresh bb ==∗ SI ∗ GC θ ∗ γ ↦imm bb)%I.
 Proof.
   iIntros "(Hσ & HGC & (Hmtζ & Hmtfresh))".
   iDestruct (GC_in_C with "Hσ HGC") as "%H"; destruct H as (ρc & mem & ->).
   iNamed "Hσ". iNamed "SIC".
-  iPoseProof (ghost_map_lookup with "HAζbl Hmtζ") as "%Hζγ".
+  iDestruct (lstore_own_mut_of with "HAζrest Hmtζ") as %[Hζγ _].
   iDestruct (lloc_own_priv_of with "HAχvirt Hmtfresh") as %Hχvirtγ.
-  iMod ((ghost_map_update (Immut,bb)) with "HAζbl Hmtζ") as "(HAζbl & Hmtζ)".
-  iMod (ghost_map_elem_persist with "Hmtζ") as "#Hmtζ".
-  iDestruct (big_sepM_insert with "[$HAζpers $Hmtζ]") as "#HAζpers2".
-  { eapply map_filter_lookup_None. right. intros ? ?. by simplify_map_eq. }
-  rewrite -lstore_immut_blocks_insert_immut //.
-  iModIntro.
-  iFrame "HGC".
-  iSplitL.
-  2: done.
-  cbn. iSplitL "HσC HnC"; first (iExists nCv; iFrame).
+  iMod (lstore_own_update _ _ _ _ (Immut,bb) with "HAζrest Hmtζ") as "(HAζrest & Hmtζ)".
+  iDestruct (lstore_own_elem_to_immut with "Hmtζ") as "Hmtζ"; first done.
+  iModIntro. iFrame "HGC Hmtζ". rewrite /= /named.
+  iSplitL "HσC HnC"; first (iExists nCv; iFrame).
   unfold C_state_interp, named.
   assert (Hζγ': ζfreeze !! γ = Some (Mut, bb)).
   { subst. rewrite lookup_union_r; eauto. by eapply map_disjoint_Some_l. }
   iExists (<[γ:=(Immut, bb)]> ζfreeze), ζσ, (<[γ:=(Immut, bb)]> ζrest).
   iExists χvirt, σMLvirt.
-  iFrame. iFrame "HAζpers2".
-  iSplitL "HAnMLv". 2: iSplitL. 3: iPureIntro; split_and!; eauto.
-  + iExists nMLv; done.
+  iFrame. iSplitL "HAnMLv"; eauto. iSplitL. 2: iPureIntro; split_and!; eauto.
   + rewrite pub_locs_in_lstore_insert_existing; eauto. by eapply elem_of_dom_2.
   + eapply freeze_lstore_freeze_lloc; eauto.
   + subst. rewrite insert_union_r. 1: done. eapply map_disjoint_Some_l; done.
@@ -189,4 +174,5 @@ Proof.
   + intros x y H. rewrite dom_insert_L. apply elem_of_union; right. by eapply Hfreezeχ.
   + eapply GC_correct_freeze_lloc; eauto.
 Qed.
+
 End UpdateLaws.
